Updates.

LC/NV/UTLC/Alpha.lean
@@ -8,40 +8,40 @@ set_option autoImplicit false
 open Term_
 
 
-inductive are_alpha_equiv : Term_ → Term_ → Prop
+inductive are_alpha_equiv_v1 : Term_ → Term_ → Prop
 
 | refl
   (M : Term_) :
-  are_alpha_equiv M M
+  are_alpha_equiv_v1 M M
 
 | symm
   (M N : Term_) :
-  are_alpha_equiv M N →
-  are_alpha_equiv N M
+  are_alpha_equiv_v1 M N →
+  are_alpha_equiv_v1 N M
 
 | trans
   (M N P : Term_) :
-  are_alpha_equiv M N →
-  are_alpha_equiv N P →
-  are_alpha_equiv M P
+  are_alpha_equiv_v1 M N →
+  are_alpha_equiv_v1 N P →
+  are_alpha_equiv_v1 M P
 
 | app
   (M M' N N' : Term_) :
-  are_alpha_equiv M M' →
-  are_alpha_equiv N N' →
-  are_alpha_equiv (app_ M N) (app_ M' N')
+  are_alpha_equiv_v1 M M' →
+  are_alpha_equiv_v1 N N' →
+  are_alpha_equiv_v1 (app_ M N) (app_ M' N')
 
 | abs
   (x : Symbol_)
   (M M' : Term_) :
-  are_alpha_equiv M M' →
-  are_alpha_equiv (abs_ x M) (abs_ x M')
+  are_alpha_equiv_v1 M M' →
+  are_alpha_equiv_v1 (abs_ x M) (abs_ x M')
 
 | alpha
   (x y : Symbol_)
   (M : Term_) :
   y ∉ M.var_set →
-  are_alpha_equiv (abs_ x M) (abs_ y (rename x y M))
+  are_alpha_equiv_v1 (abs_ x M) (abs_ y (rename x y M))
 
 
 -------------------------------------------------------------------------------
@@ -49,51 +49,51 @@ inductive are_alpha_equiv : Term_ → Term_ → Prop
 
 -- [2]
 
-inductive are_alpha_equiv_alt : Term_ → Term_ → Prop
+inductive are_alpha_equiv_v2 : Term_ → Term_ → Prop
 
 | rename
   (x y : Symbol_)
   (M : Term_) :
   y ∉ M.var_set →
-  are_alpha_equiv_alt (abs_ x M) (abs_ y (replace_free x (var_ y) M))
+  are_alpha_equiv_v2 (abs_ x M) (abs_ y (replace_free x (var_ y) M))
 
 | compat_app_left
   (M N L : Term_) :
-  are_alpha_equiv_alt M N →
-  are_alpha_equiv_alt (app_ M L) (app_ N L)
+  are_alpha_equiv_v2 M N →
+  are_alpha_equiv_v2 (app_ M L) (app_ N L)
 
 | compat_app_right
   (M N L : Term_) :
-  are_alpha_equiv_alt M N →
-  are_alpha_equiv_alt (app_ L M) (app_ L N)
+  are_alpha_equiv_v2 M N →
+  are_alpha_equiv_v2 (app_ L M) (app_ L N)
 
 | compat_abs
   (x : Symbol_)
   (M N : Term_) :
-  are_alpha_equiv_alt M N →
-  are_alpha_equiv_alt (abs_ x M) (abs_ x N)
+  are_alpha_equiv_v2 M N →
+  are_alpha_equiv_v2 (abs_ x M) (abs_ x N)
 
 | refl
   (M : Term_) :
-  are_alpha_equiv_alt M M
+  are_alpha_equiv_v2 M M
 
 | symm
   (M N : Term_) :
-  are_alpha_equiv_alt M N →
-  are_alpha_equiv_alt N M
+  are_alpha_equiv_v2 M N →
+  are_alpha_equiv_v2 N M
 
 | trans
   (L M N : Term_) :
-  are_alpha_equiv_alt L M →
-  are_alpha_equiv_alt M N →
-  are_alpha_equiv_alt L N
+  are_alpha_equiv_v2 L M →
+  are_alpha_equiv_v2 M N →
+  are_alpha_equiv_v2 L N
 
 
 lemma are_alpha_equiv_rename_replace_free
   (u v : Symbol_)
   (e : Term_)
   (h1 : v ∉ e.var_set) :
-  are_alpha_equiv (rename u v e) (replace_free u (var_ v) e) :=
+  are_alpha_equiv_v1 (rename u v e) (replace_free u (var_ v) e) :=
   by
     induction e
     case var_ x =>
@@ -103,7 +103,7 @@ lemma are_alpha_equiv_rename_replace_free
       unfold replace_free
       split_ifs
       all_goals
-        apply are_alpha_equiv.refl
+        apply are_alpha_equiv_v1.refl
     case app_ M N ih_1 ih_2 =>
       unfold var_set at h1
       simp at h1
@@ -112,7 +112,7 @@ lemma are_alpha_equiv_rename_replace_free
       specialize ih_2 h1_right
       unfold rename
       unfold replace_free
-      apply are_alpha_equiv.app
+      apply are_alpha_equiv_v1.app
       · exact ih_1
       · exact ih_2
     case abs_ x M ih =>
@@ -125,11 +125,11 @@ lemma are_alpha_equiv_rename_replace_free
       split_ifs
       case pos c1 =>
         subst c1
-        obtain s1 := are_alpha_equiv.alpha u v M h1_left
-        apply are_alpha_equiv.symm
+        obtain s1 := are_alpha_equiv_v1.alpha u v M h1_left
+        apply are_alpha_equiv_v1.symm
         exact s1
       case neg c1 =>
-        apply are_alpha_equiv.abs
+        apply are_alpha_equiv_v1.abs
         exact ih
 
 
@@ -137,7 +137,7 @@ lemma are_alpha_equiv_alt_replace_free_rename
   (u v : Symbol_)
   (e : Term_)
   (h1 : v ∉ e.var_set) :
-  are_alpha_equiv_alt (replace_free u (var_ v) e) (rename u v e) :=
+  are_alpha_equiv_v2 (replace_free u (var_ v) e) (rename u v e) :=
   by
     induction e
     case var_ x =>
@@ -147,7 +147,7 @@ lemma are_alpha_equiv_alt_replace_free_rename
       unfold replace_free
       split_ifs
       all_goals
-        apply are_alpha_equiv_alt.refl
+        apply are_alpha_equiv_v2.refl
     case app_ M N ih_1 ih_2 =>
       unfold var_set at h1
       simp at h1
@@ -156,9 +156,9 @@ lemma are_alpha_equiv_alt_replace_free_rename
       specialize ih_2 h1_right
       unfold rename
       unfold replace_free
-      obtain s1 := are_alpha_equiv_alt.compat_app_right _ _ _ ih_2
-      obtain s2 := are_alpha_equiv_alt.compat_app_left (replace_free u (var_ v) M) (rename u v M) (rename u v N) ih_1
-      apply are_alpha_equiv_alt.trans _ _ _ s1 s2
+      obtain s1 := are_alpha_equiv_v2.compat_app_right _ _ _ ih_2
+      obtain s2 := are_alpha_equiv_v2.compat_app_left (replace_free u (var_ v) M) (rename u v M) (rename u v N) ih_1
+      apply are_alpha_equiv_v2.trans _ _ _ s1 s2
     case abs_ x M ih =>
       unfold var_set at h1
       simp at h1
@@ -169,72 +169,72 @@ lemma are_alpha_equiv_alt_replace_free_rename
       split_ifs
       case pos c1 =>
         subst c1
-        obtain s1 := are_alpha_equiv_alt.rename u v M h1_left
-        apply are_alpha_equiv_alt.trans (abs_ u M) (abs_ v (replace_free u (var_ v) M)) (abs_ v (rename u v M)) s1
-        apply are_alpha_equiv_alt.compat_abs
+        obtain s1 := are_alpha_equiv_v2.rename u v M h1_left
+        apply are_alpha_equiv_v2.trans (abs_ u M) (abs_ v (replace_free u (var_ v) M)) (abs_ v (rename u v M)) s1
+        apply are_alpha_equiv_v2.compat_abs
         exact ih
       case neg c1 =>
-        apply are_alpha_equiv_alt.compat_abs
+        apply are_alpha_equiv_v2.compat_abs
         exact ih
 
 
 lemma are_alpha_equiv_imp_are_alpha_equiv_alt
   (e e' : Term_)
-  (h1 : are_alpha_equiv e e') :
-  are_alpha_equiv_alt e e' :=
+  (h1 : are_alpha_equiv_v1 e e') :
+  are_alpha_equiv_v2 e e' :=
   by
     induction h1
     case refl M =>
-      exact are_alpha_equiv_alt.refl M
+      exact are_alpha_equiv_v2.refl M
     case symm M N _ ih_2 =>
-      exact are_alpha_equiv_alt.symm M N ih_2
+      exact are_alpha_equiv_v2.symm M N ih_2
     case trans M N P _ _ ih_3 ih_4 =>
-      exact are_alpha_equiv_alt.trans M N P ih_3 ih_4
+      exact are_alpha_equiv_v2.trans M N P ih_3 ih_4
     case app M M' N N' _ _ ih_3 ih_4 =>
-      obtain s1 := are_alpha_equiv_alt.compat_app_left M M' N ih_3
-      obtain s2 := are_alpha_equiv_alt.compat_app_right N N' M' ih_4
-      exact are_alpha_equiv_alt.trans (app_ M N) (app_ M' N) (app_ M' N') s1 s2
+      obtain s1 := are_alpha_equiv_v2.compat_app_left M M' N ih_3
+      obtain s2 := are_alpha_equiv_v2.compat_app_right N N' M' ih_4
+      exact are_alpha_equiv_v2.trans (app_ M N) (app_ M' N) (app_ M' N') s1 s2
     case abs x M M' _ ih_2 =>
-      exact are_alpha_equiv_alt.compat_abs x M M' ih_2
+      exact are_alpha_equiv_v2.compat_abs x M M' ih_2
     case alpha x y M ih_1 =>
-      obtain s1 := are_alpha_equiv_alt.rename x y M ih_1
-      apply are_alpha_equiv_alt.trans (abs_ x M) (abs_ y (replace_free x (var_ y) M)) (abs_ y (rename x y M)) s1
-      apply are_alpha_equiv_alt.compat_abs y (replace_free x (var_ y) M) (rename x y M)
+      obtain s1 := are_alpha_equiv_v2.rename x y M ih_1
+      apply are_alpha_equiv_v2.trans (abs_ x M) (abs_ y (replace_free x (var_ y) M)) (abs_ y (rename x y M)) s1
+      apply are_alpha_equiv_v2.compat_abs y (replace_free x (var_ y) M) (rename x y M)
       apply are_alpha_equiv_alt_replace_free_rename; exact ih_1
 
 
 lemma are_alpha_equiv_alt_imp_are_alpha_equiv
   (e e' : Term_)
-  (h1 : are_alpha_equiv_alt e e') :
-  are_alpha_equiv e e' :=
+  (h1 : are_alpha_equiv_v2 e e') :
+  are_alpha_equiv_v1 e e' :=
   by
     induction h1
     case rename x y M ih_1 =>
-      obtain s1 := are_alpha_equiv.alpha x y M ih_1
-      apply are_alpha_equiv.trans _ _ _ s1
-      apply are_alpha_equiv.abs
+      obtain s1 := are_alpha_equiv_v1.alpha x y M ih_1
+      apply are_alpha_equiv_v1.trans _ _ _ s1
+      apply are_alpha_equiv_v1.abs
       apply are_alpha_equiv_rename_replace_free; exact ih_1
     case compat_app_left M N L _ ih_2 =>
-      apply are_alpha_equiv.app M N L L
+      apply are_alpha_equiv_v1.app M N L L
       · exact ih_2
-      · exact are_alpha_equiv.refl L
+      · exact are_alpha_equiv_v1.refl L
     case compat_app_right M N L _ ih_2 =>
-      apply are_alpha_equiv.app L L M N
-      · exact are_alpha_equiv.refl L
+      apply are_alpha_equiv_v1.app L L M N
+      · exact are_alpha_equiv_v1.refl L
       · exact ih_2
     case compat_abs x M N _ ih_2 =>
-      exact are_alpha_equiv.abs x M N ih_2
+      exact are_alpha_equiv_v1.abs x M N ih_2
     case refl M =>
-      exact are_alpha_equiv.refl M
+      exact are_alpha_equiv_v1.refl M
     case symm M N _ ih_2 =>
-      exact are_alpha_equiv.symm M N ih_2
+      exact are_alpha_equiv_v1.symm M N ih_2
     case trans M N P _ _ ih_3 ih_4 =>
-      exact are_alpha_equiv.trans M N P ih_3 ih_4
+      exact are_alpha_equiv_v1.trans M N P ih_3 ih_4
 
 
 lemma are_alpha_equiv_iff_are_alpha_equiv_alt
   (e e' : Term_) :
-  are_alpha_equiv e e' ↔ are_alpha_equiv_alt e e' :=
+  are_alpha_equiv_v1 e e' ↔ are_alpha_equiv_v2 e e' :=
   by
     constructor
     · exact are_alpha_equiv_imp_are_alpha_equiv_alt e e'
@@ -243,7 +243,7 @@ lemma are_alpha_equiv_iff_are_alpha_equiv_alt
 
 example
   (e e' : Term_)
-  (h1 : are_alpha_equiv e e') :
+  (h1 : are_alpha_equiv_v1 e e') :
   e.free_var_set = e'.free_var_set :=
   by
     induction h1
